tstack: Prove tstack impl w.r.t. spec

src/example/TreiberStackSpec.v
@@ -76,19 +76,13 @@ Section SPEC.
       phys_list n h L ∗ LInv n k γs h m
   )%S.
 
-  Definition IsT n s k γs : sProp n := (
-    syn_inv n treiberN (Inv n s k γs)
+  Definition IsT n Lay s k γs : sProp n := (
+    ◆[k,Lay] ∗ syn_inv n treiberN (Inv n s k γs)
   )%S.
 
-  Global Instance IsT_persistent n s k γs :
-    Persistent (⟦ IsT n s k γs, n⟧).
-  Proof. unfold Persistent,IsT. rewrite red_syn_inv. by iIntros "#?". Qed.
-
-  (* Lemma isSpinlock_unfold n x γx γe k L :
-    (⟦isSpinlock n x γx γe k L, n⟧) -∗ (◆[k, L] ∗ inv n N_Spinlock (spinlockInv n x γx γe)).
-  Proof.
-    iEval (unfold isSpinlock; red_tl). iIntros "[LO INV]". eauto.
-  Qed. *)
+  Global Instance IsT_persistent n L s k γs :
+    Persistent (⟦ IsT n L s k γs, n⟧).
+  Proof. unfold Persistent,IsT. red_tl. rewrite red_syn_inv. by iIntros "#?". Qed.
 
   Lemma Inv_unfold n s k γs :
     (⟦ Inv n s k γs, n ⟧) -∗
@@ -186,7 +180,7 @@ Section SPEC.
     ⊢ [@ tid, n, ⊤ @]
           ⧼⟦(
             (syn_tgt_interp_as n sndl (fun m => s_memory_black m))
-            ∗ (⤉ IsT n s k γs)
+            ∗ (⤉ IsT n lv s k γs)
             ∗ (⤉ Duty(tid) ds)
             ∗ (⤉ P)
             ∗ (∀ (S : τ{list SCMem.val, 1+n}), (⤉ (● γs (S : list SCMem.val) ∗ P))
@@ -194,7 +188,7 @@ Section SPEC.
               )
             ∗ ◇[k](1,1)
             (* TODO: Proper ord level. *)
-            ∗ ◇{List.map fst ds}(2 + lv, 1)
+            ∗ ◇{List.map fst ds}(4 + lv, 1)
             )%S, 1+n⟧⧽
             (OMod.close_itree Client (SCMem.mod gvs) (TreiberStack.push (s,val)))
           ⧼_, ⟦(
@@ -203,35 +197,53 @@ Section SPEC.
   .
   Proof.
     ii. iStartTriple. red_tl_all.
-    unfold IsT. rewrite red_syn_tgt_interp_as. rewrite red_syn_inv. simpl.
-    iIntros "(#Mem & #IsT & Duty & P & AU & Ob_k & Pcs) Post".
+    unfold IsT. rewrite red_syn_tgt_interp_as. red_tl. rewrite red_syn_inv. simpl.
+    iIntros "(#Mem & #[Ob_kb IsT] & Duty & P & AU & Ob_ks & PCS) Post".
     red_tl_all.
     iEval (unfold TreiberStack.push).
 
-    iMod (pcs_drop _ _ _ _ 1 (100 + 1) with "Pcs") as "Pcs"; [lia|].
-    Unshelve. 2: lia.
     rred2r.
 
-    iMod ((pcs_decr _ _ 100 1) with "Pcs") as "[Pcs Pcs_Y]"; [lia|].
-    iApply (wpsim_yieldR with "[$Duty $Pcs_Y]"); [lia..|].
+    iMod (pcs_drop _ _ 1 _ (3+lv) 3 with "[$PCS]") as "PCS"; [lia|].
+    iMod (pcs_decr _ _ 1 2 with "PCS") as "[Ys PCS]"; [done|].
+    iMod (pcs_decr _ _ 1 1 with "PCS") as "[PCS' PCS]"; [done|].
+    iMod (pcs_drop _ _ 1 _ 1 100 with "Ys") as "Ys"; [lia|].
+    iMod (pcs_decr _ _ 1 99 with "Ys") as "[Y Ys]"; [lia|].
+    Unshelve. 2,3: lia.
+
+    iApply (wpsim_yieldR with "[$Duty $Y]"); [lia|].
     iIntros "Duty _". rred2r.
+
+    iMod (ccs_make _ _ _ 2 1 with "[$Ob_kb PCS']") as "[CCS _]".
+    { simpl. iFrame. }
 
     iApply (SCMem_alloc_fun_spec with "[$Mem] [-]"); [lia|set_solver|].
     iIntros (node) "(n.n↦ & n.d↦ & _)".
     rred2r. iApply wpsim_tauR. rred2r.
 
-    iMod ((pcs_decr _ _ 99 1) with "Pcs") as "[Pcs Pcs_Y]"; [lia|].
-    iApply (wpsim_yieldR with "[$Pcs_Y $Duty]"); [lia|].
-    iIntros "Duty _".
-    rred2r.
+    iMod ((pcs_decr _ _ 98 1) with "Ys") as "[Ys Y]"; [lia|].
+    iApply (wpsim_yieldR with "[$Y $Duty]"); [lia|].
+    iIntros "Duty _". rred2r.
 
     iApply (SCMem_store_fun_spec with "[$Mem $n.d↦] [-]"); [lia|set_solver|].
     iIntros (?) "n.d↦". rred2r. iApply wpsim_tauR. rred2r.
 
-    iEval (rewrite unfold_iter_eq). rred2r.
+    move: (SCMem.val_nat 0) => next.
 
-    iMod ((pcs_decr _ _ 98 1) with "Pcs") as "[Pcs Pcs_Y]"; [lia|].
-    iApply (wpsim_yieldR with "[$Pcs_Y $Duty]"); [lia|].
+    iRevert "n.n↦ Post Duty Ys AU P n.d↦ Ob_ks". iRevert (next). iRevert "PCS".
+
+    iMod (ccs_ind2 with "CCS [-]") as "Ind".
+    2:{ iIntros "PCS". iMod (pcs_drop _ _ _ _ 2 1 with "PCS") as "PCS"; [lia|].
+        iApply ("Ind" with "PCS").
+    }
+    Unshelve. 2: lia.
+
+    (* TODO: is this exists 0 correct? *)
+    iModIntro. iExists 0. iIntros "IH !> Pcs %next n.n↦ Post Duty Ys AU P n.d↦ Ob_ks".
+    iEval (rewrite unfold_iter_eq). rred2r.
+    iMod ((pcs_decr _ _ 97 1) with "Ys") as "[Ys Y]"; [lia|].
+
+    iApply (wpsim_yieldR with "[$Y $Duty]"); [lia|].
     iIntros "Duty _". rred2r.
 
     iInv "IsT" as "Inv" "Close". simpl.
@@ -258,19 +270,18 @@ Section SPEC.
 
     iApply wpsim_tauR. rred2r.
 
-    iMod ((pcs_decr _ _ 97 1) with "Pcs") as "[Pcs Pcs_Y]"; [lia|].
-    iApply (wpsim_yieldR with "[$Pcs_Y $Duty]"); [lia|].
+    iMod ((pcs_decr _ _ 96 1) with "Ys") as "[Ys Y]"; [lia|].
+    iApply (wpsim_yieldR with "[$Y $Duty]"); [lia|].
     iIntros "Duty _". rred2r.
 
     iApply (SCMem_store_fun_spec with "[$Mem $n.n↦] [-]"); [lia|solve_ndisj|].
     iIntros (?) "n.n↦". rred2r. iApply wpsim_tauR. rred2r.
 
-    iMod ((pcs_decr _ _ 96 1) with "Pcs") as "[Pcs Pcs_Y]"; [lia|].
-    iApply (wpsim_yieldR with "[$Pcs_Y $Duty]"); [lia|].
-    iIntros "Duty _".
-    rred2r.
+    iMod ((pcs_decr _ _ 95 1) with "Ys") as "[Ys Y]"; [lia|].
+    iApply (wpsim_yieldR with "[$Y $Duty]"); [lia|].
+    iIntros "Duty _". rred2r.
 
-    iMod ((pcs_decr _ _ 95 1) with "Pcs") as "[Pcs Pcs_Y]"; [lia|].
+    iMod ((pcs_decr _ _ 94 1) with "Ys") as "[Ys Y]"; [lia|].
 
     iInv "IsT" as "Inv" "Close". simpl.
     iDestruct (Inv_unfold with "Inv") as (h' L m) "(s↦ & γs & Phys & LInv)".
@@ -310,9 +321,9 @@ Section SPEC.
       iMod (ghost_map_delete with "GMap i↪") as "GMap".
 
       (** Create a big_opM of ◇[k](0,1). *)
-      iMod (pc_drop _ 0 _ _ (size (delete i m)) with "Ob_k") as "Ob_k"; [lia|].
+      iMod (pc_drop _ 0 _ _ (size (delete i m)) with "Ob_ks") as "Ob_ks"; [lia|].
       Unshelve. 2: lia.
-      iAssert ([∗ map] _ ∈ delete i m, ◇[k](0,1))%I with "[Ob_k]" as "Ob_k".
+      iAssert ([∗ map] _ ∈ delete i m, ◇[k](0,1))%I with "[Ob_ks]" as "Ob_ks".
       { set (m' := delete i m). move: m' => m'.
         iClear "Mem IsT n.n↦ n.d↦". clear.
         simpl in *.
@@ -320,14 +331,14 @@ Section SPEC.
         { done. }
         rewrite big_sepM_insert; [|done].
         rewrite map_size_insert_None; [|done].
-        iDestruct (pc_split _ _ 1 (size m) with "Ob_k") as "[$ Ob_k]".
-        iApply ("IH" with "Ob_k").
+        iDestruct (pc_split _ _ 1 (size m) with "Ob_ks") as "[$ Ob_ks]".
+        iApply ("IH" with "Ob_ks").
       }
 
       (** Add it to the invariant. *)
       iDestruct (big_sepM_delete with "LivC") as "[_ LivC]"; [apply Lookup_i|].
-      iDestruct (LInv_fold _ _ _ (to_mnp_ptr node IsPtr) with "GMap [LivC Ob_k]") as "LInv".
-      { iDestruct (big_sepM_sep_2 with "LivC Ob_k") as "LivC".
+      iDestruct (LInv_fold _ _ _ (to_mnp_ptr node IsPtr) with "GMap [LivC Ob_ks]") as "LInv".
+      { iDestruct (big_sepM_sep_2 with "LivC Ob_ks") as "LivC".
         iApply (big_sepM_mono with "LivC").
         iIntros (i' p' Lookup_i') "[H C]". des_ifs.
       }
@@ -336,7 +347,7 @@ Section SPEC.
       { unfold to_val. iFrame. }
       iMod ("Close" with "Inv") as "_". rred2r.
 
-      iApply (wpsim_yieldR with "[$Pcs_Y $Duty]"); [lia|].
+      iApply (wpsim_yieldR with "[$Y $Duty]"); [lia|].
       iIntros "Duty _". rred2r. iApply wpsim_tauR. rred2r.
       iApply "Post". iFrame.
     }
@@ -356,36 +367,36 @@ Section SPEC.
       assert (Ph = Ph') as -> by apply proof_irrelevance. done.
     }
 
-    (* Update liveness invariant *)
+    (* Update ◇[k](0,1) to use for induction *)
     iDestruct (LInv_unfold with "LInv") as "[GMap LivC]".
 
     iDestruct (ghost_map_lookup with "GMap i↪") as "%Lookup_i".
     iMod (ghost_map_delete with "GMap i↪") as "GMap".
 
-    iDestruct (big_sepM_delete with "LivC") as "[iC LivC]"; [apply Lookup_i|].
+    iDestruct (big_sepM_delete with "LivC") as "[Ob_k LivC]"; [apply Lookup_i|].
     case_decide; [done|].
     red_tl. simpl.
-    (* TODO: uhh... now what? actually set up induction and stuff. *)
 
     iDestruct (LInv_fold with "GMap LivC") as "LInv".
     iDestruct (Inv_fold with "s↦ γs Phys LInv") as "Inv".
     iMod ("Close" with "Inv") as "_". rred2r.
 
     iApply wpsim_tauR. rred2r. iApply wpsim_tauR.
-  Admitted.
-(*
-∀ (S : τ{list SCMem.val}), (⤉ (● γs (S : list SCMem.val) ∗ P))
-                  =|1+n|={E}=∗
-                  (∃ (S' : τ{list SCMem.val}) (ov : τ{option SCMem.val}),
-                    (⤉ (● γs (S' : list SCMem.val) ∗ Q (ov : option SCMem.val) ∗ ⌜ov = hd_error S⌝)))
-*)
+
+    (* Do Induction *)
+    iMod (pcs_drop _ _ 1 _ 1 98 with "[$Pcs]") as "Pcs"; [lia|].
+    Unshelve. 2: lia.
+    iMod ("IH" with "Ob_k n.n↦ Post Duty Pcs AU P n.d↦ Ob_ks") as "IH".
+    iApply "IH".
+  Qed.
+
   Lemma Treiber_pop_spec
         {n} (Q : (option SCMem.val) → sProp n) (P : sProp n) tid :
-    ∀ s k γs L (ds : list (nat * nat * sProp n)),
+    ∀ s k γs lv (ds : list (nat * nat * sProp n)),
     ⊢ [@ tid, n, ⊤ @]
           ⧼⟦(
             (syn_tgt_interp_as n sndl (fun m => s_memory_black m))
-            ∗ (⤉ IsT n s k γs)
+            ∗ (⤉ IsT n lv s k γs)
             ∗ (⤉ Duty(tid) ds)
             ∗ (⤉ P)
             (* TODO: masks? *)
@@ -396,8 +407,8 @@ Section SPEC.
                   | h::t => (⤉ (● γs t ∗ Q (Some h)))
                   end
               )
-            (* TODO: Proper ord level. *)
-            ∗ ◇{List.map fst ds}(2 + L, 1)
+            ∗ ◇[k](1,1)
+            ∗ ◇{List.map fst ds}(4 + lv, 1)
             )%S, 1+n⟧⧽
             (OMod.close_itree Client (SCMem.mod gvs) (TreiberStack.pop s))
           ⧼rv, ⟦(
@@ -405,7 +416,238 @@ Section SPEC.
             )%S, 1+n⟧⧽
   .
   Proof.
-  Admitted.
+    ii. iStartTriple. red_tl_all.
+    unfold IsT. rewrite red_syn_tgt_interp_as. red_tl. rewrite red_syn_inv. simpl.
+    iIntros "(#Mem & #[Ob_kb IsT] & Duty & P & AU & Ob_ks & PCS) Post".
+    red_tl_all.
+
+    iMod (pcs_drop _ _ 1 _ (3+lv) 3 with "[$PCS]") as "PCS"; [lia|].
+    iMod (pcs_decr _ _ 1 2 with "PCS") as "[Ys PCS]"; [done|].
+    iMod (pcs_decr _ _ 1 1 with "PCS") as "[PCS' PCS]"; [done|].
+    iMod (pcs_drop _ _ 1 _ 1 102 with "Ys") as "Ys"; [lia|].
+    Unshelve. 2,3: lia.
+    iMod (ccs_make _ _ _ 2 1 with "[$Ob_kb PCS']") as "[CCS _]".
+    { simpl. iFrame. }
+
+    iEval (unfold TreiberStack.pop). rred2r.
+
+    iMod ((pcs_decr _ _ 101 1) with "Ys") as "[Ys Y]"; [lia|].
+    iApply (wpsim_yieldR with "[$Duty $Y]"); [lia..|].
+    iIntros "Duty _". rred2r.
+
+    iApply wpsim_tauR. rred2r.
+
+    iRevert "Post Duty Ys AU P Ob_ks". iRevert "PCS".
+
+    iMod (ccs_ind2 with "CCS [-]") as "Ind".
+    2:{ iIntros "PCS". iMod (pcs_drop _ _ _ _ 2 1 with "PCS") as "PCS"; [lia|].
+        iApply ("Ind" with "PCS").
+    }
+    Unshelve. 2: lia.
+
+    iModIntro. iExists 0. iIntros "IH !> PCS Post Duty Ys AU P Ob_ks".
+    iEval (rewrite unfold_iter_eq). rred2r.
+
+    iMod ((pcs_decr _ _ 100 1) with "Ys") as "[Ys Y]"; [lia|].
+    iApply (wpsim_yieldR with "[$Duty $Y]"); [lia..|].
+    iIntros "Duty _". rred2r.
+
+    iInv "IsT" as "Inv" "Close". simpl.
+    iDestruct (Inv_unfold with "Inv") as (h St m) "(s↦ & γs & Phys & LInv)".
+
+    iApply (SCMem_load_fun_spec with "[$Mem $s↦] [-]"); [lia|solve_ndisj|].
+    iIntros (?) "[%EQ s↦]".
+    subst. rred2r. iApply wpsim_tauR. rred2r.
+    iMod ((pcs_decr _ _ 99 1) with "Ys") as "[Ys Y]"; [lia|].
+
+    destruct (decide (to_val h = to_mnp_null)) as [EQ|NEQ].
+    { (* Head is null, so stack is empty. *)
+      destruct h as [[h|h] EQh]; ss.
+      subst. injection EQ as ->. simpl in *.
+      iEval (rewrite phys_list_unfold) in "Phys".
+      des_ifs; last first.
+      { iDestruct "Phys" as (p r) "[%EQ _]". simpl in EQ. done. }
+      iClear "Phys".
+      iSpecialize ("AU" $! []). iEval (red_tl; rewrite red_syn_fupd; red_tl_all) in "AU".
+      iMod ("AU" with "[$γs $P]") as "[γs Q]".
+      iDestruct (Inv_fold with "[s↦] γs [] LInv") as "Inv".
+      { unfold to_val. iFrame. }
+      { iApply phys_list_fold. done. }
+      iMod ("Close" with "Inv") as "_". rred2r.
+
+      iApply (wpsim_yieldR with "[$Duty $Y]"); [lia..|].
+      iIntros "Duty _". rred2r.
+
+      iApply (SCMem_compare_fun_spec with "[Mem] [-]"); [|solve_ndisj| |].
+      2:{ iApply (tgt_interp_as_equiv with "Mem"). clear.
+          iStartProof. iIntros (m). simpl. red_tl_all. iSplit.
+          - iIntros "$". iPureIntro. done.
+          - iIntros "[$ _]".
+        }
+      1: lia.
+      iIntros (?) "%EQ". destruct EQ as [EQ _]. des; last done.
+      specialize (EQ EQh) as ->. rred2r.
+
+      iApply (wpsim_tauR). rred2r.
+      iApply "Post". red_tl_all. iFrame.
+    }
+
+    iDestruct (phys_list_get_head with "Phys") as "#h↦□".
+    case_decide; [done|].
+    iDestruct "h↦□" as (r d) "[h.n↦□ [h.d↦□ _]]".
+    (* Update Linv by adding myself to the ghost map, in the same way as push *)
+
+    iDestruct (LInv_unfold with "LInv") as "[GMap LivC]".
+    set (i := fresh (dom m)).
+    iMod (ghost_map_insert i h with "[$GMap]") as "[GMap i↪]".
+    { apply not_elem_of_dom. apply is_fresh. }
+
+    iDestruct (LInv_fold with "GMap [LivC]") as "LInv".
+    { rewrite big_sepM_insert; last first.
+      { apply not_elem_of_dom. apply is_fresh. }
+      iFrame. case_decide; done.
+    }
+
+    iDestruct (Inv_fold with "s↦ γs Phys LInv") as "Inv".
+    iMod ("Close" with "Inv") as "_". move: i=>i. clear dependent St m.
+
+    iApply (wpsim_yieldR with "[$Duty $Y]"); [lia..|].
+    iIntros "Duty _". rred2r.
+
+    iApply (SCMem_compare_loc_null_fun_spec with "[$Mem $h.n↦□] [-]"); [lia|solve_ndisj|].
+    iIntros (?) "[_ %EQ]". subst. rred2r.
+
+    iApply (wpsim_tauR). rred2r.
+
+    iMod ((pcs_decr _ _ 98 1) with "Ys") as "[Ys Y]"; [lia|].
+    iApply (wpsim_yieldR with "[$Duty $Y]"); [lia..|].
+    iIntros "Duty _". rred2r.
+
+    iApply (SCMem_load_fun_spec with "[$Mem $h.n↦□] [-]"); [lia|solve_ndisj|].
+    iIntros (?) "[%EQ _]". subst. rred2r.
+
+    iApply (wpsim_tauR). rred2r.
+
+    iMod ((pcs_decr _ _ 97 1) with "Ys") as "[Ys Y]"; [lia|].
+    iApply (wpsim_yieldR with "[$Duty $Y]"); [lia..|].
+    iIntros "Duty _". rred2r.
+
+    iInv "IsT" as "Inv" "Close". simpl.
+    iDestruct (Inv_unfold with "Inv") as (h' L m) "(s↦ & γs & Phys & LInv)".
+    iDestruct (phys_list_get_head with "Phys") as "#h'↦□".
+    destruct (decide (h = h')) as [<-|NEQhh'].
+    { des_ifs. iDestruct "h'↦□" as (r' d') "[h'.n↦□ [h'.d↦□ _]]". subst.
+      iDestruct (memory_ra_points_to_agree with "h.d↦□ h'.d↦□") as %<-.
+      iDestruct (memory_ra_points_to_agree with "h.n↦□ h'.n↦□") as %<-.
+
+      iDestruct (phys_list_unfold with "Phys") as "Phys".
+      destruct L as [|v tL].
+      { iDestruct "Phys" as %EQ. done. }
+      iDestruct "Phys" as (? r_new) "[%EQ_p [[#h.n↦□' [#h.d↦□' _]] Phys]]".
+
+      iDestruct (memory_ra_points_to_agree with "h.d↦□ h.d↦□'") as %<-.
+      iDestruct (memory_ra_points_to_agree with "h.n↦□ h.n↦□'") as %->.
+      clear r. iClear "h.n↦□' h.d↦□' h'.n↦□ h'.d↦□".
+
+      (* Equal, CAS success *)
+      iApply (SCMem_cas_loc_fun_spec_gen with "[$Mem $s↦] [-]"); [lia|solve_ndisj| |].
+      { des_ifs.
+        iSplit; iExists _; iFrame "h.n↦□".
+      }
+      iIntros (b) "POST".
+
+      iDestruct "POST" as (u) "(%EQ & s↦ & _ & _)".
+      des_ifs. destruct EQ as [-> ->].
+      iSpecialize ("AU" $! (d::tL)).
+      iEval (red_tl) in "AU".
+      iEval (rewrite red_syn_fupd) in "AU".
+      iEval (red_tl_all) in "AU".
+      rred2r. iApply wpsim_tauR. rred2r.
+
+      (* Update logical & physical stack state. *)
+      iMod ("AU" with "[$γs $P]") as "[γs Q]".
+
+      (* Update liveness invariant *)
+      iDestruct (LInv_unfold with "LInv") as "[GMap LivC]".
+
+      iDestruct (ghost_map_lookup with "GMap i↪") as "%Lookup_i".
+      iMod (ghost_map_delete with "GMap i↪") as "GMap".
+
+      (** Create a big_opM of ◇[k](0,1). *)
+      iMod (pc_drop _ 0 _ _ (size (delete i m)) with "Ob_ks") as "Ob_ks"; [lia|].
+      Unshelve. 2: lia.
+      iAssert ([∗ map] _ ∈ delete i m, ◇[k](0,1))%I with "[Ob_ks]" as "Ob_ks".
+      { set (m' := delete i m). move: m' => m'.
+        iClear "Mem IsT h.n↦□ h.d↦□ Ob_kb". clear.
+        simpl in *.
+        iInduction (m') as [|id op m NotIN] "IH" using map_ind.
+        { done. }
+        rewrite big_sepM_insert; [|done].
+        rewrite map_size_insert_None; [|done].
+        iDestruct (pc_split _ _ 1 (size m) with "Ob_ks") as "[$ Ob_ks]".
+        iApply ("IH" with "Ob_ks").
+      }
+
+      (** Add it to the invariant. *)
+      iDestruct (big_sepM_delete with "LivC") as "[_ LivC]"; [apply Lookup_i|].
+      iDestruct (LInv_fold _ _ _ r_new with "GMap [LivC Ob_ks]") as "LInv".
+      { iDestruct (big_sepM_sep_2 with "LivC Ob_ks") as "LivC".
+        iApply (big_sepM_mono with "LivC").
+        iIntros (i' p' Lookup_i') "[H C]". des_ifs.
+      }
+
+      iDestruct (Inv_fold with "s↦ γs Phys LInv") as "Inv".
+      iMod ("Close" with "Inv") as "_". rred2r.
+
+      iMod ((pcs_decr _ _ 96 1) with "Ys") as "[Ys Y]"; [lia|].
+      iApply (wpsim_yieldR with "[$Y $Duty]"); [lia|].
+      iIntros "Duty _". rred2r.
+
+      iApply (SCMem_load_fun_spec with "[$Mem $h.d↦□] [-]"); [lia|solve_ndisj|].
+      iIntros (?) "[%EQ _]". subst. rred2r.
+
+      iApply wpsim_tauR. rred2r.
+
+      iApply "Post". red_tl. iFrame.
+    }
+    (* Different, CAS fail *)
+    iApply (SCMem_cas_loc_fun_spec_gen with "[$Mem $s↦ h.n↦□ h'↦□] [-]"); [lia|solve_ndisj| |].
+    { unfold to_val. des_ifs.
+      2: iDestruct "h'↦□" as (??) "[h'↦□ _]".
+      all: iSplit; try done; iExists _; iFrame "#".
+    }
+    iClear "h'↦□".
+    iIntros (b) "POST". iDestruct "POST" as (u) "(%EQ & s↦ & _ & _)".
+    destruct (SCMem.val_eq_dec (to_val h') (to_val h)).
+    all: destruct EQ as [-> ->].
+    { exfalso. unfold to_val in e. apply NEQhh'.
+      destruct h,h'. simpl in *. subst. f_equal. apply proof_irrelevance.
+    }
+
+    (* Update ◇[k](0,1) to use for induction *)
+    iDestruct (LInv_unfold with "LInv") as "[GMap LivC]".
+
+    iDestruct (ghost_map_lookup with "GMap i↪") as "%Lookup_i".
+    iMod (ghost_map_delete with "GMap i↪") as "GMap".
+
+    iDestruct (big_sepM_delete with "LivC") as "[Ob_k LivC]"; [apply Lookup_i|].
+    case_decide; [done|].
+    red_tl. simpl.
+
+    iDestruct (LInv_fold with "GMap LivC") as "LInv".
+    iDestruct (Inv_fold with "s↦ γs Phys LInv") as "Inv".
+    iMod ("Close" with "Inv") as "_". rred2r.
+
+    iApply wpsim_tauR. rred2r.
+
+    iApply wpsim_tauR. rred2r.
+
+    (* Do Induction *)
+    iMod (pcs_drop _ _ 1 _ 1 101 with "[$PCS]") as "PCS"; [lia|].
+    Unshelve. 2: lia.
+    iMod ("IH" with "Ob_k Post Duty PCS AU P Ob_ks") as "IH".
+    iApply "IH".
+Qed.
 
 End SPEC.
 
